

Normal Distribution

Normal Distribution by definition

Standardized Normal Distribution

$$Z \sim \mathcal{N}(0, 1), \quad f_Z(z) = \frac{1}{\sqrt{2\pi}} e^{-z^2/2}$$

$$\mathbb{E}[Z] = \int_{-\infty}^{\infty} z f_Z(z) dz = \frac{1}{\sqrt{2\pi}} \int_{-\infty}^{\infty} z e^{-z^2/2} dz = \left\| \begin{array}{l} u = -\frac{z^2}{2} \\ du = -z dz \end{array} \right\| = \frac{1}{\sqrt{2\pi}} \int_{-\infty}^{\infty} e^u du = \frac{e^u}{\sqrt{2\pi}} \Big|_{-\infty}^{\infty} = 0$$

$$\begin{aligned} \mathbb{E}[Z^2] &= \int_{-\infty}^{\infty} z^2 f_Z(z) dz = \frac{1}{\sqrt{2\pi}} \int_{-\infty}^{\infty} z^2 e^{-z^2/2} dz = \left\| \begin{array}{l} u = z, \quad du = dz \\ dv = z e^{-z^2/2} dz, \quad v = -e^{-z^2/2} \end{array} \right\| \\ &= \frac{1}{\sqrt{2\pi}} \left(-z e^{-z^2/2} \Big|_{-\infty}^{\infty} - \int_{-\infty}^{\infty} (-e^{-z^2/2}) dz \right) = \frac{1}{\sqrt{2\pi}} \left(0 + \int_{-\infty}^{\infty} e^{-z^2/2} dz \right) = 1 \end{aligned}$$

$$\text{Var}[Z] = \mathbb{E}[Z^2] - (\mathbb{E}[Z])^2 = 1 - 0 = 1$$

$$X \sim \mathcal{N}(\mu, \sigma^2)$$

$$Z = \frac{X - \mu}{\sigma} \Rightarrow X = \sigma Z + \mu$$

$$\mathbb{E}[X] = \mathbb{E}[\sigma Z + \mu] = \sigma \times 0 + \mu = \mu$$

$$\text{Var}(X) = \text{Var}(\sigma Z + \mu) = \sigma^2 \times \text{Var}(Z) = \sigma^2 \times 1 = \sigma^2$$

Moment-generating function of Normal Distribution

$$Z \sim \mathcal{N}(0, 1), \quad f_Z(z) = \frac{1}{\sqrt{2\pi}} e^{-z^2/2}$$

$$\begin{aligned} M_Z(t) &= \mathbb{E}[e^{tz}] = \int_{-\infty}^{\infty} e^{tz} f_Z(z) dz = \frac{1}{\sqrt{2\pi}} \int_{-\infty}^{\infty} e^{tz} e^{-z^2/2} dz = \frac{1}{\sqrt{2\pi}} \int_{-\infty}^{\infty} e^{tz - z^2/2} dz = \\ &= \left\| tz - \frac{z^2}{2} = \frac{2tz}{2} - \frac{z^2}{2} = -\frac{1}{2}(z^2 - 2tz) = -\frac{1}{2}((z-t)^2 - t^2) = -\frac{(z-t)^2}{2} + \frac{t^2}{2} \right\| \\ &= \frac{1}{\sqrt{2\pi}} \int_{-\infty}^{\infty} e^{-\frac{(z-t)^2}{2} + \frac{t^2}{2}} dz = \frac{1}{\sqrt{2\pi}} \int_{-\infty}^{\infty} e^{-\frac{(z-t)^2}{2}} \times e^{\frac{t^2}{2}} dz = \\ &= e^{\frac{t^2}{2}} \int_{-\infty}^{\infty} \underbrace{\frac{1}{\sqrt{2\pi}} e^{-\frac{(z-t)^2}{2}}}_{=1 \text{ pdf of } \mathcal{N}(t, 1)} dz = e^{\frac{t^2}{2}} \end{aligned}$$

$$X \sim \mathcal{N}(\mu, \sigma^2), \quad X = \sigma * Z + \mu, \quad Z \sim \mathcal{N}(0, 1)$$

$$M_X(t) = \mathbb{E}[e^{tX}] = \mathbb{E}[e^{t(\sigma Z + \mu)}] = \mathbb{E}[e^{t\sigma Z + t\mu}] = e^{\mu t} \times \mathbb{E}[e^{t\sigma Z}] = e^{\mu t} \times M_Z(\sigma t) = e^{\mu t} \times e^{\frac{(\sigma t)^2}{2}} = e^{\mu t + \frac{(\sigma t)^2}{2}}$$

@salyamq

@salyamq

@salyamq

@salyamq
@salyamq
@salyamq
@salyamq
@salyamq
@salyamq
@salyamq
@salyamq
@salyamq
@salyamq
@salyamq
@salyamq
@salyamq
@salyamq
@salyamq
@salyamq
@salyamq
@salyamq